Cl is finite symm logic

Foundation/Propositional/Kripke/Hilbert/Cl.lean
@@ -1,6 +1,9 @@
 import Foundation.Propositional.Hilbert.WellKnown
-import Foundation.Propositional.Kripke.Hilbert.Soundness
 import Foundation.Propositional.Kripke.AxiomLEM
+import Foundation.Propositional.Kripke.AxiomWeakLEM
+import Foundation.Propositional.Kripke.Filteration
+import Foundation.Propositional.Kripke.Hilbert.Soundness
+import Foundation.Propositional.Kripke.Rooted
 
 namespace LO.Propositional
 
@@ -11,18 +14,45 @@ open Formula.Kripke
 namespace Kripke.FrameClass
 
 protected abbrev euclidean : FrameClass := { F | IsEuclidean _ F }
+protected abbrev finite_symmetric : FrameClass := { F | Finite F ∧ IsSymm _ F }
+protected abbrev finite_euclidean : FrameClass := { F | Finite F ∧ IsEuclidean _ F }
+
+lemma eq_finite_euclidean_finite_symmetric : FrameClass.finite_euclidean = FrameClass.finite_symmetric := by
+  ext F;
+  constructor;
+  . rintro ⟨_, hF⟩; exact ⟨by tauto, inferInstance⟩;
+  . rintro ⟨_, hF⟩; exact ⟨by tauto, inferInstance⟩;
 
 end Kripke.FrameClass
 
 
 namespace Hilbert.Cl.Kripke
 
-instance sound : Sound Hilbert.Cl FrameClass.euclidean :=
+instance sound_finite : Sound Hilbert.Cl FrameClass.finite_symmetric :=
+  instSound_of_validates_axioms $ by
+    apply FrameClass.Validates.withAxiomEFQ;
+    rintro F ⟨_, hF⟩ _ rfl;
+    apply validate_LEM_of_symmetric;
+
+instance sound_finite_symmetric : Sound Hilbert.Cl FrameClass.finite_symmetric :=
+  instSound_of_validates_axioms $ by
+    apply FrameClass.Validates.withAxiomEFQ;
+    rintro F ⟨_, hF⟩ _ rfl;
+    apply validate_LEM_of_symmetric;
+
+instance sound_euclidean : Sound Hilbert.Cl FrameClass.euclidean :=
   instSound_of_validates_axioms $ by
     apply FrameClass.Validates.withAxiomEFQ;
     rintro F hF _ rfl;
     replace hF := Set.mem_setOf_eq.mp hF;
     apply validate_LEM_of_euclidean;
+
+instance sound_finite_euclidean : Sound Hilbert.Cl FrameClass.finite_euclidean :=
+  instSound_of_validates_axioms $ by
+    apply FrameClass.Validates.withAxiomEFQ;
+    rintro F ⟨_, hF⟩ _ rfl;
+    apply validate_LEM_of_euclidean;
+
 
 instance consistent : Entailment.Consistent Hilbert.Cl := consistent_of_sound_frameclass FrameClass.euclidean $ by
   use whitepoint;
@@ -35,6 +65,54 @@ instance canonical : Canonical Hilbert.Cl FrameClass.euclidean :=  ⟨by
 ⟩
 
 instance complete : Complete Hilbert.Cl FrameClass.euclidean := inferInstance
+
+section FFP
+
+open
+  finestFilterationTransitiveClosureModel
+  Relation
+
+instance complete_finite_symmetric : Complete (Hilbert.Cl) FrameClass.finite_symmetric := ⟨by
+  intro φ hφ;
+  apply Kripke.complete.complete;
+  rintro F F_con V r;
+  replace F_con := Set.mem_setOf_eq.mp F_con;
+  let M : Kripke.Model := ⟨F, V⟩;
+  let RM := M↾r;
+
+  apply Model.pointGenerate.modal_equivalent_at_root (M := M) (r := r) |>.mp;
+
+  let FRM := finestFilterationTransitiveClosureModel RM (φ.subformulas);
+  apply filteration FRM finestFilterationTransitiveClosureModel.filterOf (by simp) |>.mpr;
+  apply hφ;
+
+  refine ⟨?_, ?_⟩;
+  . apply FilterEqvQuotient.finite; simp;
+  . apply isSymm_iff _ _ |>.mpr;
+    rintro ⟨x, (rfl | Rrx)⟩ ⟨y, (rfl | Rry)⟩ RXY;
+    . simp_all;
+    . apply TransGen.single;
+      use ⟨y, by tauto⟩, ⟨x, by tauto⟩;
+      refine ⟨by tauto, by tauto, ?_⟩;
+      . have : y ≺ x := IsSymm.symm _ _ Rry;
+        tauto;
+    . apply TransGen.single;
+      use ⟨y, by tauto⟩, ⟨x, by tauto⟩;
+      refine ⟨by tauto, by tauto, ?_⟩;
+      . have : x ≺ y := IsSymm.symm _ _ Rrx;
+        tauto;
+    . apply Relation.TransGen.single;
+      use ⟨y, by tauto⟩, ⟨x, by tauto⟩;
+      refine ⟨by tauto, by tauto, ?_⟩;
+      . have : y ≺ x := IsEuclidean.euclidean Rrx Rry;
+        tauto;
+⟩
+
+instance complete_finite_euclidean : Complete (Hilbert.Cl) FrameClass.finite_euclidean := by
+  convert complete_finite_symmetric;
+  exact FrameClass.eq_finite_euclidean_finite_symmetric;
+
+end FFP
 
 end Hilbert.Cl.Kripke
 
